working add instruction

SP1Operations/AddOperationNew.lean
@@ -1,4 +1,6 @@
 import SP1Foundations
+import LeanRV32D.RiscvInstsEnd
+import LeanRV32D.RiscvRegs
 
 -- Probably good to still namespace things
 namespace AddOperation
@@ -161,3 +163,104 @@ lemma bitVecAdd_of_addOperationConstraintSet
 end corollary
 
 end AddOperation
+
+namespace Add
+
+-- Add below imports to the top of the file
+/- import LeanRV32D.RiscvInstsEnd -/
+/- import LeanRV32D.RiscvRegs -/
+
+open LeanRV32D.Functions
+open Sail
+open PreSail (SequentialState)
+
+open AddOperation
+
+def AddChipConstraints
+    (Input0 Input1 Input2 Input3 Input4 Input5 Input6 : BabyBear) : Finset SP1Constraint :=
+  AddOperationConstraints Input0 Input1 Input2 Input3 Input4 Input5 Input6
+
+def sp1_add
+  -- All the columns used for `AddChip` (currently includes only those from `add_operation`)
+  (Input0 Input1 Input2 Input3 Input4 Input5 Input6 : BabyBear)
+  (constraints :
+    constraintSet_toProp (AddOperationConstraints Input0 Input1 Input2 Input3 Input4 Input5 Input6))
+  -- the following 4 proofs will come from the spec/constraints of `RTypeReader`
+  -- adding in manually for now
+  (read_b0_constraint : Input0.val < 65536) 
+  (read_b1_constraint : Input1.val < 65536)
+  (read_c0_constraint : Input2.val < 65536)
+  (read_c1_constraint : Input3.val < 65536)
+  -- ensures this is not a padding row (we're actually running the instruction)
+  (h' : Input6 ≠ 0)
+  -- registers to read/write
+  (rd rs1 rs2 : regidx)
+  : SailM Unit := 
+  -- the human part of the code generation is to fill out the `pf`s
+  let Input0 : U16 := ⟨Input0, read_b0_constraint⟩
+  let Input1 : U16 := ⟨Input1, read_b1_constraint⟩
+  let Input2 : U16 := ⟨Input2, read_c0_constraint⟩
+  let Input3 : U16 := ⟨Input3, read_c1_constraint⟩
+  let hh :=
+    AddOperationSpec_of_AddOperationConstraintSet Input0 Input1 Input2 Input3 _ _ _ constraints
+  let pf : Input4.val + Input5.val * 65536 < 2^32 := by
+    have ⟨hb, ⟨hc, _⟩⟩ := (hh.right h')
+    omega
+
+  -- below will be auto-generated
+  do
+    writeReg Register.nextPC (BitVec.addInt (← readReg Register.PC) 4)
+    let _ ← rX_bits rs1
+    let _ ← rX_bits rs2
+    -- at code-gen time, we don't know whether `Input4 + Input5 * 65536` will
+    -- be in `u32` range, so we leave out the placeholder for us to manually
+    -- fill in
+    wX_bits rd (BitVec.ofNatLT (Input4.val + Input5.val * 65536) pf)
+
+/- noncomputable -/ def spec_add (rd rs1 rs2 : regidx) : SailM Unit := do
+  writeReg Register.nextPC (BitVec.addInt (← readReg Register.PC) 4)
+  /- let _ ← execute (.RTYPE ⟨rs2, rs1, rd, rop.ADD⟩) -/ -- `execute` is uncomputable...?
+  let _ ← execute_RTYPE rs2 rs1 rd rop.ADD
+  pure ()
+
+theorem sp1_add_implies_spec_add
+  (Input0 Input1 Input2 Input3 Input4 Input5 Input6 : BabyBear)
+  (constraints :
+    constraintSet_toProp (AddOperationConstraints Input0 Input1 Input2 Input3 Input4 Input5 Input6))
+  -- the following 4 proofs will come from the spec/constraints of `RTypeReader`
+  -- adding in manually for now
+  (read_b0_constraint : Input0.val < 65536) 
+  (read_b1_constraint : Input1.val < 65536)
+  (read_c0_constraint : Input2.val < 65536)
+  (read_c1_constraint : Input3.val < 65536)
+  -- ensures this is not a padding row (we're actually running the instruction)
+  (h_is_real : Input6 ≠ 0)
+  (rd rs1 rs2 : regidx)
+  (read_b_fun : rX_bits rs1 = pure (BitVec.ofU16 ⟨Input0, read_b0_constraint⟩ ⟨Input1, read_b1_constraint⟩))
+  (read_c_fun : rX_bits rs2 = pure (BitVec.ofU16 ⟨Input2, read_c0_constraint⟩ ⟨Input3, read_c1_constraint⟩))
+  (s : PreSail.SequentialState RegisterType trivialChoiceSource)
+  : let res := (sp1_add _ _ _ _ _ _ _ constraints read_b0_constraint read_b1_constraint read_c0_constraint read_c1_constraint h_is_real rd rs1 rs2).run s 
+    let res_spec := (spec_add rd rs1 rs2).run s
+  res = res_spec :=
+  by
+    let Input0 : U16 := ⟨Input0, read_b0_constraint⟩
+    let Input1 : U16 := ⟨Input1, read_b1_constraint⟩
+    let Input2 : U16 := ⟨Input2, read_c0_constraint⟩
+    let Input3 : U16 := ⟨Input3, read_c1_constraint⟩
+    simp [EStateM.run]
+    simp [sp1_add, spec_add, /- execute, -/ execute_RTYPE]
+    let h_bv :=
+      bitVecAdd_of_addOperationConstraintSet
+      (Input0 := Input0)
+      (Input1 := Input1)
+      (Input2 := Input2)
+      (Input3 := Input3)
+      constraints
+      h_is_real
+    rw [←h_bv]
+    rw [read_b_fun, read_c_fun]
+    clear h_bv read_b_fun read_c_fun
+    rw [pure_bind, pure_bind]
+    rfl
+
+end Add
